\documentclass[11pt]{article}
\textwidth 15cm 
\textheight 21.3cm
\evensidemargin 6mm
\oddsidemargin 6mm
\topmargin -1.1cm
\setlength{\parskip}{1.5ex}


\usepackage{amsfonts,amsmath,amssymb,enumerate}

\begin{document}
\parindent=0pt


\begin{align*}
L_b(b)+ L_b(a) & = L_a(a) + L_a(b)\\
f(b)+f'(b)(b-b)+f(b)+f'(b)(a-b) & =  f(a)+f'(a)(a-a)+f(a)+f'(a)(b-a)\\
f(b)+f(b)+f'(b)(-(b-a)) & = f(a)+f(a)+f'(a)(b-a)\\
2f(b)-f'(b)(b-a)  &= 2f(a)+ f'(a)(b-a)\\
2f(b) - 2f(a) &= f'(b)(b-a) + f'(a)(b-a)\\
2(f(b) - f(a)) &= (f'(b) + f'(a))(b-a)\\
\frac{f(b)-f(a)}{b-a} &= \frac{f'(b)+f'(a)}{2}
\end{align*}







\end{document}